% Problem 2.3 Solution
We now turn our attention to solving equation (\ref{odebeta}). To do this, we first solve the homogeneous equation, 
\begin{equation}
    \beta_n'' - \gamma_n^2 \beta_n = 0,
    \label{odebeta}
\end{equation}
by assuming a solution of the form $\beta_n(z) = e^{\lambda_n z}$. Substituting our ansatz into equation (\ref{odebeta}) yields the characteristic polynomial.
\begin{equation}
    \lambda_n^2 e^{\lambda_n z} - \gamma_n^2 e^{\lambda_n z} = 0 \implies \lambda_n = \pm\gamma_n
\end{equation}
Hence, the general solution to the homogeneous problem can be written as follows.
\begin{align}
    \beta_n^H(z) &= a e^{-\lambda_n z} + b e^{\lambda_n z}\\
    &= a e^{-\gamma_n z} + b e^{\gamma_n z}
\end{align}
However, we may also write the general solution in terms of a different set of linearly independent functions. Recall that the hyperbolic sine and cosine functions are linear combinations of the exponential functions, $e^x$ and $e^{-x}$.
\begin{align}
    \sinh(x) &= \frac{1}{2}\left(e^{x} - e^{-x}\right)\\
    \cosh(x) &= \frac{1}{2}\left(e^{x} + e^{-x}\right)
\end{align}
Hence, if we let $x = \gamma_n z$, we may, without loss of generality, write the general solution to the homogeneous problem as 
\begin{equation}
    \boxed{\beta_n^H(z) = c_1 \sinh(\gamma_n z) + c_2 \cosh(\gamma_n z).}
\end{equation}