\begin{solution}
	Since $w^h, v^h \in V^h$, let 
	\begin{align}
		w^h &= \sum_{A=1}^n w_A N_A(x) \\
		v^h &= \sum_{B=1}^n u_B N_B(x) \\
		g^h &= u_0 N_{n+1}(x) \\
		u^h &= v^h + g^h = \sum_{B=1}^n u_B N_B(x) + u_0 N_{n+1}(x)
	\end{align}
	where $N_A(0) = 0, N_B (0) = 0, N_{n+1}(0) = 1$. Substitute Eq.(105-108) into the Galerkin statement, we have
	\begin{gather}
			a\int_0^1 \left(\sum_{A=1}^n w_A N_A(x)\right) \partial_{x}\left( \sum_{B=1}^n u_B N_B(x) \right) dx - \lambda \int_0^1 \left(\sum_{A=1}^n w_A N_A(x)\right) \left( \sum_{B=1}^n u_B N_B(x) \right) dx \notag \\
			+ k \int_0^1 \partial_{x}\left(\sum_{A=1}^n w_A N_A(x)\right) \partial_{x}\left( \sum_{B=1}^n u_B N_B(x) \right) dx \notag \\
		= \int_0^1 \left(\sum_{A=1}^n w_A N_A(x)\right) f dx + \left(\sum_{A=1}^n w_A N_A(1)\right)b_1 - a\int_0^1 \left(\sum_{A=1}^n w_A N_A(x)\right) \partial_{x}\left( u_0 N_{n+1}(x) \right) dx \notag \\
		+ \lambda \int_0^1 \left(\sum_{A=1}^n w_A N_A(x)\right) \left( u_0 N_{n+1}(x) \right) dx - k \int_0^1 \partial_{x}\left(\sum_{A=1}^n w_A N_A(x)\right) \partial_{x}\left( u_0 N_{n+1}(x) \right) dx
	\end{gather}
	Denote the basis functions $N_A(x)$ and $N_B(x)$ to be nonnegative, by the Fubini Theorem, we can simplify Eq.(109) into
	\begin{align}
		\sum_{A=1}^n w_A & \left( a\int_0^1 N_A(x) \partial_{x} \left( \sum_{B=1}^n u_B N_B(x) \right) dx - \lambda \int_0^1 N_A(x) \left( \sum_{B=1}^n u_B N_B(x) \right) dx \notag \right. \notag \\
		&+ k \int_0^1 \partial_{x}\left(N_A(x)\right) \partial_{x}\left( \sum_{B=1}^n u_B N_B(x) \right) dx - \int_0^1 f N_A dx - N_A(1) b_1 \notag \\
		&+ a \int_0^1 N_A(x) \partial_{x}\left( u_0 N_{n+1}(x) \right) dx - \lambda u_0 \int_0^1 N_A(x) N_{n+1}(x) dx \notag \\
		&\left. + k u_0 \int_0^1 \partial_{x}(N_A(x)) \partial_{x}(N_{n+1}(x)) dx \right) = 0
	\end{align}
	To satisfy Eq.(110), the terms in the bracket must be zero:
	\begin{gather}
		a\int_0^1 N_A(x) \partial_{x} \left( \sum_{B=1}^n u_B N_B(x) \right) dx - \lambda \int_0^1 N_A(x) \left( \sum_{B=1}^n u_B N_B(x) \right) dx \notag \\
		+ k \int_0^1 \partial_{x}\left(N_A(x)\right) \partial_{x}\left( \sum_{B=1}^n u_B N_B(x) \right) dx - \int_0^1 f N_A dx - N_A(1) b_1 \notag \\
		+ a \int_0^1 N_A(x) \partial_{x}\left( u_0 N_{n+1}(x) \right) dx - \lambda u_0 \int_0^1 N_A(x) N_{n+1}(x) dx \notag \\
		+ k u_0 \int_0^1 \partial_{x}(N_A(x)) \partial_{x}(N_{n+1}(x)) dx = 0
	\end{gather}
	By applying the Fubini Theorem again, we have
	\begin{gather}
	    \sum_{B=1}^n a\int_0^1 N_A(x) \partial_{x} \left( u_B N_B(x) \right) dx - \sum_{B=1}^n \lambda \int_0^1 N_A(x) \left( u_B N_B(x) \right) dx \notag \\
	    + \sum_{B=1}^n k \int_0^1 \partial_{x}\left(N_A(x)\right) \partial_{x}\left( u_B N_B(x) \right) dx \notag \\
	    = \int_0^1 f N_A dx + N_A(1) b_1 - a \int_0^1 N_A(x) \partial_{x}\left( u_0 N_{n+1}(x) \right) dx \notag \\
	    + \lambda u_0 \int_0^1 N_A(x) N_{n+1}(x) - k u_0 \int_0^1 \partial_{x}(N_A(x)) \partial_{x}(N_{n+1}(x)) dx
	\end{gather}
	Denote the series and integrals in Eq.(112) as
	\begin{align}
	    \sum_{B=1}^n A_{AB} u_B &= \sum_{B=1}^n a\int_0^1 N_A(x) \partial_{x} \left( u_B N_B(x) \right) dx \\
	    \sum_{B=1}^n \Lambda_{AB} u_B &= \sum_{B=1}^n \lambda \int_0^1 N_A(x) \left( u_B N_B(x) \right) dx \\
	    \sum_{B=1}^n K_{AB} u_B &= \sum_{B=1}^n k \int_0^1 \partial_{x}\left(N_A(x)\right) \partial_{x}\left( u_B N_B(x) \right) dx \\
	    F_A &= \int_0^1 f N_A dx + N_A(1) b_1 - a \int_0^1 N_A(x) \partial_{x}\left( u_0 N_{n+1}(x) \right) dx \notag \\
	    &+ \lambda u_0 \int_0^1 N_A(x) N_{n+1}(x) - k u_0 \int_0^1 \partial_{x}(N_A(x)) \partial_{x}(N_{n+1}(x)) dx
	\end{align}
	where
	\begin{align}
	    A_{AB} &= \int_0^1 N_A(x) \partial_{x} \left( N_B(x) \right) dx \\
	    \Lambda_{AB} &= \int_0^1 N_A(x) \left( N_B(x) \right) dx \\
	    K_{AB} &= \int_0^1 \partial_{x}\left(N_A(x)\right) \partial_{x}\left( N_B(x) \right) dx
	\end{align}
		
		
	\begin{tcolorbox}
		We reach the linear algebra problem: Solve for
		\begin{equation*}
		    \sum_{B=1}^n a A_{AB}u_B - \sum_{B=1}^n \lambda \Lambda_{AB}u_B	+ \sum_{B=1}^n k K_{AB}u_B = F_A, A = 1, \cdots, n
		\end{equation*}
		where $A_{AB}, \Lambda_{AB}, K_{AB}, F_A$ are denoted in Eq.(116-119).
	\end{tcolorbox}
	
\end{solution}